p4cub type system refactor

deps/poulet4/lib/Utils/Util/FunUtil.v
@@ -87,3 +87,24 @@ Definition
   | inl a => inl (f a)
   | inr b => inr (g b)
   end.
+
+Section OExists.
+  Context {A : Set}.
+  Variable P : A -> Prop.
+
+  Variant OExists : option A -> Prop :=
+    OExist_some a :
+      P a -> OExists (Some a).
+
+  Local Hint Constructors OExists : core.
+
+  Lemma OExists_exists : forall o : option A,
+      OExists o <-> exists a, P a /\ o = Some a.
+  Proof.
+    intros [a |]; split.
+    - intro h; inv h; eauto.
+    - intros (a' & H & h); inv h; auto.
+    - intro h; inv h.
+    - intros (a' & H & h); inv h.
+  Qed.
+End OExists.
